Add views for UInt8/16/32 + clean up

src/arch/x64/Views.fst
@@ -31,3 +31,63 @@ assume val put64 (a:UInt64.t) : GTot (Seq.lseq UInt8.t 8)
 assume val inverses64 (u:unit) : Lemma (inverses get64 put64)
 
 let view64 = inverses64 (); View 8 get64 put64
+
+let get8 (s:Seq.lseq UInt8.t 1) = Seq.index s 0
+let put8 (x:UInt8.t) : GTot (Seq.lseq UInt8.t 1) =
+  let contents (i:nat{i<1}) = x in
+  Seq.init 1 contents
+
+let inverses8 (u:unit) : Lemma (inverses get8 put8) =
+  let aux (x:Seq.lseq UInt8.t 1) : Lemma (put8 (get8 x) == x) =
+    assert (Seq.equal x (put8 (get8 x)))
+  in Classical.forall_intro aux
+
+let view8 = inverses8 (); View 1 get8 put8
+
+let get16 (s:Seq.lseq UInt8.t 2) = UInt16.uint_to_t (
+  UInt8.v (Seq.index s 0) + 
+  UInt8.v (Seq.index s 1) `op_Multiply` 0x100
+  )
+let put16 (x:UInt16.t) : GTot (Seq.lseq UInt8.t 2) =
+  let s = Seq.create 2 (UInt8.uint_to_t 0) in
+  let x = UInt16.v x in
+  let s = Seq.upd s 0 (UInt8.uint_to_t (x % 0x100)) in
+  let x = x `op_Division` 0x100 in
+  let s = Seq.upd s 1 (UInt8.uint_to_t (x % 0x100)) in
+  s
+
+let inverses16 (u:unit) : Lemma (inverses get16 put16) =
+  let aux (x:Seq.lseq UInt8.t 2) : Lemma (put16 (get16 x) == x) =
+    assert (Seq.equal x (put16 (get16 x)))
+  in Classical.forall_intro aux
+
+let view16 = inverses16 (); View 2 get16 put16
+
+let get32 (s:Seq.lseq UInt8.t 4) = UInt32.uint_to_t (
+  UInt8.v (Seq.index s 0) + 
+  UInt8.v (Seq.index s 1) `op_Multiply` 0x100 +
+  UInt8.v (Seq.index s 2) `op_Multiply` 0x10000 +
+  UInt8.v (Seq.index s 3) `op_Multiply` 0x1000000  
+  )
+let put32 (x:UInt32.t) : GTot (Seq.lseq UInt8.t 4) =
+  let s = Seq.create 4 (UInt8.uint_to_t 0) in
+  let x = UInt32.v x in
+  let s = Seq.upd s 0 (UInt8.uint_to_t (x % 0x100)) in
+  let x = x `op_Division` 0x100 in
+  let s = Seq.upd s 1 (UInt8.uint_to_t (x % 0x100)) in
+  let x = x `op_Division` 0x100 in
+  let s = Seq.upd s 2 (UInt8.uint_to_t (x % 0x100)) in
+  let x = x `op_Division` 0x100 in
+  let s = Seq.upd s 3 (UInt8.uint_to_t (x % 0x100)) in
+  s
+
+#set-options "--z3rlimit 20"
+
+let inverses32 (u:unit) : Lemma (inverses get32 put32) =
+  let aux (x:Seq.lseq UInt8.t 4) : Lemma (put32 (get32 x) == x) =
+    assert (Seq.equal x (put32 (get32 x)))
+  in Classical.forall_intro aux
+
+let view32 = inverses32(); View 4 get32 put32
+
+assume val view128: (v:view UInt8.t quad32{View?.n v == 16})
